reference/Operational/Awkernel/GeneratedHandoffTraceArtifact.v
@@ -3,11 +3,11 @@ From RocqSched Require Import Operational.Common.Step.
 From RocqSched Require Import Operational.Awkernel.Minimal.CapturedTraceSyntax.
 Import ListNotations.
 
-Definition awk_generated_handoff_rows : list AwkernelCapturedRow :=
-  [ mkAwkernelCapturedRow 0 (EvWakeup 1) None [1] false None
-  ; mkAwkernelCapturedRow 1 (EvRequestResched 1) None [1] true None
-  ; mkAwkernelCapturedRow 1 (EvHandleResched 1) None [1] true None
-  ; mkAwkernelCapturedRow 1 (EvChoose 1 1) None [1] true (Some 1)
-  ; mkAwkernelCapturedRow 1 (EvDispatch 1 1) (Some 1) [] false None
-  ; mkAwkernelCapturedRow 1 (EvComplete 1) None [] true None
+Definition awk_generated_handoff_rows : list AwkernelSchedTraceEntry :=
+  [ mkAwkernelSchedTraceEntry 0 (EvWakeup 1) None [1] false None
+  ; mkAwkernelSchedTraceEntry 1 (EvRequestResched 1) None [1] true None
+  ; mkAwkernelSchedTraceEntry 1 (EvHandleResched 1) None [1] true None
+  ; mkAwkernelSchedTraceEntry 1 (EvChoose 1 1) None [1] true (Some 1)
+  ; mkAwkernelSchedTraceEntry 1 (EvDispatch 1 1) (Some 1) [] false None
+  ; mkAwkernelSchedTraceEntry 1 (EvComplete 1) None [] true None
   ].
