theories/Operational/Awkernel/Minimal/WorkloadAcceptanceExtraction.v
@@ -5,6 +5,7 @@ From RocqSched Require Import Operational.Awkernel.Minimal.WorkloadAcceptance.
 Extraction Language Haskell.
 
 Extraction "/scheduling_theory/extracted/haskell/AwkernelWorkloadAcceptance.hs"
-  TaskLifecycleKind
-  TaskLifecycleRecord
-  awk_workload_accepts_trace.
+  AwkernelTaskTraceKind
+  AwkernelTaskTraceEntry
+  AwkernelSchedTraceEntry
+  awk_workload_accepts_sched_trace.
